op_a_one case

SP1Chips/JalChip.lean
@@ -13,52 +13,56 @@ def constraints (Main : Vector (Fin BB) 31) : SP1ConstraintList :=
   let E6 : Fin BB := E3 + 8
   let E7 : Fin BB := Main[2] - 1
   let E8 : Fin BB := E7 * 1761607681
-  let E9 : Fin BB := Main[30] - Main[13]
-  let CS1 : SP1ConstraintList := AddOperation.constraints #v[Main[3], Main[4], Main[5], 0] #v[4, 0, 0, 0] { value := #v[Main[26], Main[27], Main[28], Main[29]] } E9
-  let E10 : Fin BB := Main[13] * Main[26]
-  let E11 : Fin BB := Main[13] * Main[27]
-  let E12 : Fin BB := Main[13] * Main[28]
-  let E13 : Fin BB := Main[1] * 65536
-  let E14 : Fin BB := Main[2] + E13
-  let E15 : Fin BB := Main[30] - 1
-  let E16 : Fin BB := Main[30] * E15
-  let E17 : Fin BB := Main[26] - 0
-  let E18 : Fin BB := Main[13] * E17
-  let E19 : Fin BB := Main[27] - 0
+  let E9 : Fin BB := Main[30] - 1
+  let E10 : Fin BB := E9 * Main[13]
+  let E11 : Fin BB := Main[30] - Main[13]
+  let CS1 : SP1ConstraintList := AddOperation.constraints #v[Main[3], Main[4], Main[5], 0] #v[4, 0, 0, 0] { value := #v[Main[26], Main[27], Main[28], Main[29]] } E11
+  let E12 : Fin BB := Main[13] * Main[26]
+  let E13 : Fin BB := Main[13] * Main[27]
+  let E14 : Fin BB := Main[13] * Main[28]
+  let E15 : Fin BB := Main[1] * 65536
+  let E16 : Fin BB := Main[2] + E15
+  let E17 : Fin BB := Main[30] - 1
+  let E18 : Fin BB := Main[30] * E17
+  let E19 : Fin BB := Main[26] - 0
   let E20 : Fin BB := Main[13] * E19
-  let E21 : Fin BB := Main[28] - 0
+  let E21 : Fin BB := Main[27] - 0
   let E22 : Fin BB := Main[13] * E21
-  let E23 : Fin BB := Main[29] - 0
+  let E23 : Fin BB := Main[28] - 0
   let E24 : Fin BB := Main[13] * E23
-  let E25 : Fin BB := E14 + 3
-  let E26 : Fin BB := Main[30] - 1
-  let E27 : Fin BB := Main[30] * E26
-  let E28 : Fin BB := E25 - Main[11]
-  let E29 : Fin BB := E28 - 1
-  let E30 : Fin BB := E29 - Main[12]
-  let E31 : Fin BB := E30 * 2013235201
+  let E25 : Fin BB := Main[29] - 0
+  let E26 : Fin BB := Main[13] * E25
+  let E27 : Fin BB := E16 + 3
+  let E28 : Fin BB := Main[30] - 1
+  let E29 : Fin BB := Main[30] * E28
+  let E30 : Fin BB := E27 - Main[11]
+  let E31 : Fin BB := E30 - 1
+  let E32 : Fin BB := E31 - Main[12]
+  let E33 : Fin BB := E32 * 2013235201
   [
     (.assertZero E1),
     (.assertZero Main[25]),
     (.assertZero E5),
     (.receive (.state Main[0] E3 Main[3] Main[4] Main[5]) Main[30]),
     (.send (.state Main[0] E6 Main[22] Main[23] Main[24]) Main[30]),
-    (.send (.byte (ByteOpcode.ofNat 7) E8 13 0) Main[30]),
+    (.send (.byte (ByteOpcode.ofNat 6) E8 13 0) Main[30]),
     (.send (.byte (ByteOpcode.ofNat 3) 0 Main[1] 0) Main[30]),
-    (.assertZero Main[29]),
     (.assertZero E10),
-    (.assertZero E11),
+    (.assertZero Main[29]),
     (.assertZero E12),
-    (.assertZero E16),
+    (.assertZero E13),
+    (.assertZero E14),
     (.assertZero E18),
+    (.send (.program Main[3] Main[4] Main[5] (Opcode.ofNat 33) Main[6] Main[14] Main[15] Main[16] Main[17] Main[18] Main[19] Main[20] Main[21] Main[13] 1 1 111 0 0) Main[30]),
     (.assertZero E20),
     (.assertZero E22),
     (.assertZero E24),
-    (.assertZero E27),
-    (.send (.byte (ByteOpcode.ofNat 7) Main[12] 16 0) Main[30]),
-    (.send (.byte (ByteOpcode.ofNat 3) 0 E31 0) Main[30]),
+    (.assertZero E26),
+    (.assertZero E29),
+    (.send (.byte (ByteOpcode.ofNat 6) Main[12] 16 0) Main[30]),
+    (.send (.byte (ByteOpcode.ofNat 3) 0 E33 0) Main[30]),
     (.send (.memory Main[0] Main[11] Main[6] 0 0 Main[7] Main[8] Main[9] Main[10]) Main[30]),
-    (.receive (.memory Main[0] E25 Main[6] 0 0 Main[26] Main[27] Main[28] Main[29]) Main[30]),
+    (.receive (.memory Main[0] E27 Main[6] 0 0 Main[26] Main[27] Main[28] Main[29]) Main[30]),
   ] ++ CS0 ++ CS1
 
 open LeanRV64IM.Functions
@@ -68,17 +72,46 @@ lemma eq_zero_of_constraints (Main : Vector (Fin BB) 31)
   simp [constraints] at h_cstrs
   aesop
 
-lemma link_eq_of_constraints (Main : Vector (Fin BB) 31)
+lemma isU64_of_constraints (Main : Vector (Fin BB) 31)
     (h_cstrs : (constraints Main).allHold)
     (h_is_real : Main[30] = 1) :
+    Word.isU64 #v[Main[3], Main[4], Main[5], 0] := by
+  simp [constraints, h_is_real, SP1Constraint.toProp] at h_cstrs
+  refine Word.isU64_of_cases ?_ ?_ ?_ ?_ ?_
+  · aesop
+  · aesop
+  · aesop
+  · aesop
+
+lemma isU64_of_constraints' (Main : Vector (Fin BB) 31)
+    (h_cstrs : (constraints Main).allHold)
+    (h_is_real : Main[30] = 1) :
+    Word.isU64 #v[Main[14], Main[15], Main[16], Main[17]] := by
+  simp [constraints, h_is_real, SP1Constraint.toProp] at h_cstrs
+  refine Word.isU64_of_cases ?_ ?_ ?_ ?_ ?_
+  · aesop
+  · aesop
+  · aesop
+  · aesop
+
+lemma link_eq_of_constraints (Main : Vector (Fin BB) 31)
+    (h_cstrs : (constraints Main).allHold)
+    (h_is_real : Main[30] = 1) (h_op_a : Main[13] = 0) :
     BitVec.ofNat 64 (Main[26] + Main[27] * 2^16 + Main[28] * 2^32 +  Main[29] * 2^48) =
       BitVec.ofNat 64 (Main[3] + Main[4] * 2^16 + Main[5] * 2^32) + 4 := by
+  have h345 := isU64_of_constraints Main h_cstrs h_is_real
   simp [constraints] at h_cstrs
   have : (AddOperation.constraints #v[Main[3], Main[4], Main[5], 0] #v[4, 0, 0, 0]
       { value := #v[Main[26], Main[27], Main[28], Main[29]] } (Main[30] - Main[13])).allHold := by
-    sorry
+    aesop
+  have := AddOperation.correct _ _ _ _ ?_ this h345 ?_
+  simp [Word.toBitVec64] at this
+  have := this.2
+  refine this.trans ?_
+  simp [Word.toNat]
+  · simp [h_op_a, h_is_real]
+  · apply Word.isU64_of_cases <;> simp
 
-  sorry
 
 lemma add_imm_eq_of_constarints (Main : Vector (Fin BB) 31)
     (h_cstrs : (constraints Main).allHold)
@@ -86,11 +119,18 @@ lemma add_imm_eq_of_constarints (Main : Vector (Fin BB) 31)
     BitVec.ofNat 64 (Main[22] + Main[23] * 65536 + Main[24] * 4294967296) =
         BitVec.ofNat 64 (Main[3] + Main[4] * 65536 + ↑Main[5] * 4294967296) +
           BitVec.ofNat 64 (Main[14] + Main[15] * 65536 + Main[16] * 4294967296 + Main[17] * 281474976710656) := by
+  have h345 := isU64_of_constraints Main h_cstrs h_is_real
+  have h1415 := isU64_of_constraints' Main h_cstrs h_is_real
   simp [constraints] at h_cstrs
   have : (AddOperation.constraints #v[Main[3], Main[4], Main[5], 0] #v[Main[14], Main[15], Main[16], Main[17]]
       { value := #v[Main[22], Main[23], Main[24], Main[25]] } Main[30]).allHold := by
-    sorry
-  sorry
+    aesop
+  have := AddOperation.correct _ _ _ _ h_is_real this h345 h1415
+  simp [Word.toBitVec64] at this
+  have := this.2
+  have h25 : Main[25] = 0 := h_cstrs.2.1
+  simp [Word.toNat, h25] at this
+  exact this
 
 lemma ofInt_ofNat_of_constraints (Main : Vector (Fin BB) 31)
     (h_cstrs : (constraints Main).allHold)
@@ -131,14 +171,8 @@ theorem SP1JAL_correct (Main : Vector (Fin BB) 31)
 
   unfold sp1Jal specJal
 
-  simp [map_eq_bind_pure_comp, execute_JAL, h_is_real]
-
   have h25 : Main[25] = 0 := by
     refine eq_zero_of_constraints Main h_cstrs
-
-  have h_link : BitVec.ofNat 64 (Main[26] + Main[27] * 2^16 + Main[28] * 2^32 +  Main[29] * 2^48) =
-      BitVec.ofNat 64 (Main[3] + Main[4] * 2^16 + Main[5] * 2^32) + 4 := by
-    refine link_eq_of_constraints Main h_cstrs h_is_real
 
   have h_imm :
       BitVec.ofNat 64 (Main[22] + Main[23] * 65536 + Main[24] * 4294967296) =
@@ -149,6 +183,41 @@ theorem SP1JAL_correct (Main : Vector (Fin BB) 31)
   have h_of_int : let imm_nat : ℕ := Main[14] + Main[15] * 65536 + Main[16] * 4294967296 + Main[17] * 281474976710656
       BitVec.ofInt 64 (BitVec.ofNat 21 (imm_nat)).toInt = (BitVec.ofNat 64 (imm_nat)) :=
     ofInt_ofNat_of_constraints Main h_cstrs h_is_real
+
+
+  have op_a_is_bool : Main[13] = 1 ∨ Main[13] = 0 := by
+
+    sorry
+
+  cases op_a_is_bool with
+  | inl op_a_is_one =>
+
+      simp [constraints, op_a_is_one, h_is_real] at h_cstrs
+      have h26 : Main[26] = 0 := by aesop
+      have h27 : Main[27] = 0 := by aesop
+      have h28 : Main[28] = 0 := by aesop
+      have h29 : Main[29] = 0 := by aesop
+      have h6 : Main[6] = 0 := by
+
+        sorry
+      simp [h25, h26, h27, h28, h29, h6]
+      rw [h_imm]
+      unfold execute_JAL
+      simp_rw [h_access]
+      simp [h25, h_ext_zca, h_pc, h_access,
+        LeanRV64IM.Functions.not, get_next_pc, bit_to_bool, bool_bit_backwards,
+        bits_of_virtaddr, ext_control_check_pc, set_next_pc,
+        sign_extend, Sail.BitVec.signExtend, BitVec.signExtend]
+      rw [h_of_int]
+      unfold wX_bits
+      simp [wX]
+  | inr op_a_is_zero =>
+
+  have h_link : BitVec.ofNat 64 (Main[26] + Main[27] * 2^16 + Main[28] * 2^32 +  Main[29] * 2^48) =
+      BitVec.ofNat 64 (Main[3] + Main[4] * 2^16 + Main[5] * 2^32) + 4 := by
+    refine link_eq_of_constraints Main h_cstrs h_is_real op_a_is_zero
+
+  simp [map_eq_bind_pure_comp, execute_JAL, h_is_real]
 
   erw [h_link]
   simp_rw [h_access]
